feat (HPGCL_Exp_run) add proof for quantitative Frame rule, proof for lemmaB1 sorried

HPGCL_Expected_Running_Time.thy
@@ -2,13 +2,13 @@
 chapter \<open>A Calculus for the expected running time of hpGCL\<close>
 theory HPGCL_Expected_Running_Time
 imports QSL_For_Potentials
- HPGCL "HOL-Eisbach.Eisbach"
+ HPGCL "HOL-Eisbach.Eisbach" "Differential_Game_Logic.Lib"
 begin
 
 
 paragraph \<open>Summary\<close>
 
-text \<open>This theory introduces the an expected running time (ERT) calculus
+text \<open>This theory introduces the expected running time (ERT) calculus
         for hpGCL.
 
       We use the ert calculus for pGCL and extend it to heap manipulating programs.
@@ -52,7 +52,7 @@ term "(P -\<star>\<^sub>p Q)"
 primrec ert :: "hpgcl \<Rightarrow> (stack \<times> heap \<Rightarrow> ennreal) \<Rightarrow> stack \<times> heap \<Rightarrow> ennreal"  where
   "ert Skip X = (\<lambda>x. X x + 1)"
 | "ert (Seq c1 c2) X = ert c1 (ert c2 X)" 
-| "ert (Coin c1 p c2) X = (\<lambda>s. p * ert c1 X s + (1-p) * ert c2 X s)"  
+(* | "ert (Coin c1 p c2) X = (\<lambda>s. p * ert c1 X s + (1-p) * ert c2 X s)"  *)
 | "ert (If b c1 c2) X = (\<lambda>(s,h). (if b s then ert c1 X (s,h) else ert c2 X (s,h)))"
 | "ert (While b c) X = lfp (\<lambda>Y (s,h). 1 + (if b s then ert c Y (s,h) else X (s,h) ))" 
 | "ert (Assign v e) X = (\<lambda>(s,h). X (s(v:=e s),h) + 1)"
@@ -68,6 +68,129 @@ primrec ert :: "hpgcl \<Rightarrow> (stack \<times> heap \<Rightarrow> ennreal) 
 
 
 
+lemma sup_continuous_ert: "sup_continuous (ert P)"
+  apply (induction P)
+  (* apply   (auto intro!: order_continuous_intros sup_continuous_lfp''[THEN sup_continuous_applyD]
+           dest: sup_continuous_compose sup_continuous_applyD) *)
+  oops
+
+ 
+
+lemma ert_If_alt: "ert (If b c1 c2) X = inf (emb\<^sub>p (\<lambda>(s,h). b s) + ert c1 X) (emb\<^sub>p (\<lambda>(s,h). \<not>b s) + ert c2 X)"
+  by(auto simp add: sup_fun_def emb\<^sub>p_alt top_add  split: if_splits prod.splits)  
+
+
+text \<open>sub-distributivity of \<open>\<star>\<^sub>p\<close> over inf \<close>
+
+lemma sub_distributivity_of_star_over_inf:
+  "(X \<star>\<^sub>p (inf Y Z)) \<ge> inf (X \<star>\<^sub>p Y) (X \<star>\<^sub>p Z)"
+  unfolding star_pot_method_alt'
+  apply(rule le_funI)
+  apply auto
+proof -
+  fix a b 
+  let ?f = "(\<lambda>(x,y). X (a, x) + Y (a, y))"
+  let ?g = "(\<lambda>(x,y). X (a, x) + Z (a, y))"
+  have "inf (Inf {X (a, x) + Y (a, y) |x y. b = x + y \<and> x ## y}) (Inf {X (a, x) + Z (a, y) |x y. b = x + y \<and> x ## y})
+    = inf (Inf (?f `{(x,y) |x y. b = x + y \<and> x ## y})) (Inf (?g ` {(x,y) |x y. b = x + y \<and> x ## y}))"
+    apply (rule arg_cong2[where f=inf]) apply(rule arg_cong[where f=Inf]) apply auto
+    apply(rule arg_cong[where f=Inf]) apply auto done
+  also have "\<dots> = (INF a\<in>{(x,y) |x y. b = x + y \<and> x ## y}. inf (?f a) (?g a))"
+    apply(subst INF_inf_distrib) by simp
+  also have "\<dots> \<le> Inf {X (a, x) + ENNREAL_PLUS.fsup Y Z (a, y) |x y. b = x + y \<and> x ## y}"
+    apply(rule Inf_mono)
+    apply auto
+    subgoal for x y
+      apply(rule exI[where x=x])
+      apply(rule exI[where x=y]) apply auto 
+      by (simp add: ENNREAL_PLUS.sup_times_distrib)
+    done
+  finally show " inf (Inf {X (a, x) + Y (a, y) |x y. b = x + y \<and> x ## y})
+                   (Inf {X (a, x) + Z (a, y) |x y. b = x + y \<and> x ## y})
+         \<le> Inf {X (a, x) + ENNREAL_PLUS.fsup Y Z (a, y) |x y. b = x + y \<and> x ## y}"
+    .
+qed
+     
+
+
+lemma sub_distributivity_of_star_over_inf':
+  "((inf Y Z) \<star>\<^sub>p X ) \<ge> inf (Y \<star>\<^sub>p X) (Z \<star>\<^sub>p X)"
+  apply(subst (3) star_pot_method_commute)    
+  apply(subst (1) star_pot_method_commute)  
+  apply(subst (2) star_pot_method_commute)
+  apply(subst sub_distributivity_of_star_over_inf)
+  by simp
+
+
+lemma ert_mono:
+  "f\<le>g \<Longrightarrow> ert c f \<le> ert c g"
+proof (induct c arbitrary: f g)
+case Skip
+  then show ?case by (auto simp: le_fun_def)
+next
+case (Assign x1 x2)
+  then show ?case by (auto simp: le_fun_def)
+next
+  case (Seq c1 c2)
+then show ?case by (auto simp: le_fun_def)
+(*next
+  case (Coin c1 x2 c2)
+  then show ?case 
+    apply (auto simp: le_fun_def)
+    apply(rule add_mono)
+    subgoal apply(rule mult_left_mono) by auto
+    subgoal apply(rule mult_left_mono) by auto
+    done *)
+next
+  case (If x1 c1 c2)
+  then show ?case 
+    by (auto simp: le_fun_def)
+next
+  case (While x1 c)
+  then show ?case 
+    apply (auto simp:  )
+    apply(rule lfp_mono) by (auto simp: le_fun_def)
+next
+  case (New x1 x2)
+  then show ?case
+    apply (auto simp: le_fun_def)
+    apply (rule Sup_mono)
+    apply safe
+    apply auto
+    subgoal for a b ab
+      apply(rule exI[where x="([(\<lambda>_. ab) \<mapsto> x2] -\<star>\<^sub>p (\<lambda>(s, h). g (s(x1 := ab), h))) (a, b)"])
+      apply safe apply(rule exI[where x=ab]) apply simp
+      apply(rule wand_pot_method_Rmono) by auto
+    done
+next
+  case (Free x)
+  then show ?case
+    by (auto simp: le_fun_def intro: star_pot_method_mono)
+next
+  case (Lookup x1 x2)
+  then show ?case
+    apply (auto simp: le_fun_def)
+    apply (rule Inf_mono)
+    apply safe 
+    apply auto
+    subgoal for a b val
+      apply(rule exI[where x=" ([x2 \<mapsto> (\<lambda>_. val)] \<star>\<^sub>p [x2 \<mapsto> (\<lambda>_. val)] -\<star>\<^sub>p (\<lambda>(s, h). f (s(x1 := val), h))) (a, b)"])
+      apply safe apply(rule exI[where x=val]) apply simp
+      apply(rule star_pot_method_mono) apply simp
+      apply(rule wand_pot_method_Rmono) by auto
+    done
+next
+  case (Update x1 x2)
+  then show ?case 
+    by (auto simp: le_fun_def intro!: star_pot_method_mono  wand_pot_method_Rmono) 
+qed 
+
+lemma ert_mono':
+  "f\<le>g \<Longrightarrow> ert c f x\<le> ert c g x"
+  using ert_mono  
+  by (simp add: le_funD)
+
+
 definition chara where
   "chara b c X Y = (\<lambda>(s,h). 1 + (if b s then ert c Y (s,h) else X (s,h)))"
 
@@ -78,6 +201,667 @@ theorem invariant_rule:
   assumes "chara b c X I \<le> I"
   shows "ert (While b c) X \<le> I"
   using assms  by(auto intro: lfp_lowerbound simp add: chara_def) 
+
+
+subsection \<open>Dollar Assertion\<close>
+
+
+definition dollar where
+  "dollar c = (\<lambda>(s,h). if h=0 then c else \<infinity>)"
+
+lemma plus_as_dollar_conv: "\<And>Q a c. Q a + c = (Q \<star>\<^sub>p dollar c) a"  
+  unfolding dollar_def star_pot_method_alt''
+  apply auto
+  apply(rule antisym)
+  subgoal apply(rule Inf_greatest) apply auto  
+    by (simp add: add_top)  
+  subgoal for Q a b apply(rule Inf_lower)
+    apply ( rule image_eqI[where x="(b,0)"]) apply simp apply simp done
+  done
+
+lemma plus_as_dollar_conv': "\<And>Q. (\<lambda>a. Q a + c) = (Q \<star>\<^sub>p dollar c)"  
+  apply (rule ext) by(rule plus_as_dollar_conv)
+
+
+lemma ert_New_alt: "ert (New x ve) X =
+     ((\<lambda>(s,h). (SUP a\<in>UNIV.  (( (pt (\<lambda>_. a) ve))  -\<star>\<^sub>p (\<lambda>(s,h). X (s(x:=a),h))) (s,h)) ) \<star>\<^sub>p dollar 1) "
+  apply simp
+  apply(rule ext)  apply simp
+  unfolding plus_as_dollar_conv[symmetric]
+  apply simp
+  apply(rule arg_cong[where f=Sup]) by auto
+
+
+lemma ert_Lookup_alt: "ert (Lookup x ae) X =
+     ((\<lambda>(s,h). (INF val\<in>UNIV.  ((pt ae (\<lambda>_. val)) \<star>\<^sub>p ( (pt ae (\<lambda>_. val)) -\<star>\<^sub>p (\<lambda>(s,h). X (s(x:=val),h)))) (s,h)
+        )) \<star>\<^sub>p dollar 1)"
+  apply simp
+  apply(rule ext)  apply simp
+  unfolding plus_as_dollar_conv[symmetric]
+  apply simp
+  apply(rule arg_cong[where f=Inf]) by auto
+
+
+subsection \<open>Hoare triples\<close>
+
+
+definition "Hoare_triple \<Phi> c \<Psi> \<equiv> \<Phi> \<ge> ert c \<Psi>"
+
+lemma Hoare_tripleI[intro]: "\<Phi> \<ge> ert c \<Psi> \<Longrightarrow> Hoare_triple \<Phi> c \<Psi>"
+  unfolding Hoare_triple_def .
+
+lemma Hoare_tripleD: "Hoare_triple \<Phi> c \<Psi> \<Longrightarrow> \<Phi> \<ge> ert c \<Psi>"
+  unfolding Hoare_triple_def .
+
+
+
+
+
+subsection \<open>Quantitative Frame Rule\<close>
+
+lemma Assign_propagates_star: "x1 \<notin> Vars \<Pi> \<Longrightarrow>
+     ((\<lambda>(s, h). \<Psi> (s(x1 := x2 s), h)) \<star>\<^sub>p \<Pi>) (a, b)
+      = ( \<Psi>  \<star>\<^sub>p \<Pi>) (a(x1 := x2 a), b)"
+  unfolding star_pot_method_alt'
+  apply simp
+  apply(rule arg_cong[where f=Inf])
+  apply auto
+  subgoal for xa y
+    apply(rule exI[where x=xa])
+    apply(rule exI[where x=y])
+    apply safe 
+    apply(drule not_in_Vars_upd_okay[where s=a and v="x2 a" and h=y]) 
+    by simp
+  subgoal for xa y
+    apply(rule exI[where x=xa])
+    apply(rule exI[where x=y])
+    apply safe 
+    apply(drule not_in_Vars_upd_okay[where s=a and v="x2 a" and h=y]) 
+    by simp 
+  done
+    
+lemma quantitative_frame_rule_aux: "(Mod c1 \<union> Mod c2) \<inter> Vars \<Pi> = {}
+    \<Longrightarrow> Mod c1  \<inter> Vars \<Pi> = {} \<and> Mod c2 \<inter> Vars \<Pi> = {}" by auto
+
+lemma theorem_3_11_3': "pure\<^sub>p X \<Longrightarrow> ((X + Y) \<star>\<^sub>p Z) = (X + (Y \<star>\<^sub>p Z))"
+  unfolding plus_fun_def
+  using theorem_3_11_3[of X Y Z]  
+  .
+
+
+lemma zz: "(a::ennreal) * Inf G \<le> (INF x\<in>G. a * x)"
+  apply(rule Inf_greatest)
+  apply auto
+  by (simp add: ENNREAL_PLUS.Sup_upper mult_left_mono)
+
+lemma zz2: "ENNREAL_PLUS.SUPR {f (x,y) |x y. ba = x + y \<and> x ## y} g
+  = ENNREAL_PLUS.SUPR {(x,y)|x y. ba = x + y \<and> x ## y} (g o f)"
+  apply auto 
+  apply(rule arg_cong[where f=Inf]) by auto
+
+(*
+lemma blab: "((\<lambda>s. a*F s+b*G s) \<star>\<^sub>p (\<lambda>s. a*F' s+b*G' s)) \<ge> (\<lambda>s. a*(F\<star>\<^sub>pF') s+b*(G\<star>\<^sub>pG') s)"
+  unfolding star_pot_method_alt'
+  apply(rule le_funI)
+  apply auto
+  apply(rule order.trans)
+   apply(rule add_mono)
+    apply(rule zz) apply(rule zz)
+  supply [[unify_trace_failure]]
+  apply(subst zz2)
+  apply(rule order.trans)
+  using ENNREAL_PLUS.SUP_times_distrib2_general
+  apply(rule ENNREAL_PLUS.SUP_times_distrib2_general)
+  sorry
+*)
+
+
+lemma qfr_aux1: "Sup ((\<lambda>x. Inf ((\<lambda>y. (f x y)::ennreal)`Y) )`X) \<le> Inf ((\<lambda>y. Sup ((\<lambda>x. f x y)`X))`Y)"
+  by (simp add: ENNREAL_PLUS.SUP_least ENNREAL_PLUS.SUP_upper SUP_mono')
+
+
+lemma star_pot_method_alt''':
+  "(P \<star>\<^sub>p Q) = (\<lambda>(s,h). INF (x,y)\<in> { (x, y). x ## y}. if  h=x+y then P(s,x) + Q(s,y) else top )"
+  unfolding star_pot_method_alt'  
+  apply(rule ext)
+  apply auto
+  apply(rule antisym)
+  subgoal
+    by (smt ENNREAL_PLUS.bot_least Inf_greatest Inf_lower imageE mem_Collect_eq split_beta) 
+  subgoal
+    apply(rule Inf_greatest)
+    apply auto apply(rule Inf_lower2)
+    by auto
+  done
+
+
+lemma SUP_to_UNIV: "(SUP h\<in>M. f h) = (SUP h\<in>UNIV. if h\<in>M then f h else (bot::'b::complete_lattice))"  
+  apply(rule antisym)
+  subgoal 
+    apply(rule Sup_least)
+    apply(rule Sup_upper2) by auto
+  subgoal    
+    by (smt SUP_least Sup_upper ccSUP_empty empty_iff image_eqI) 
+  done
+
+lemma INF_to_UNIV: "(INF h\<in>M. f h) = (INF h\<in>UNIV. if h\<in>M then f h else (top::'b::complete_lattice))"  
+  apply(rule antisym)
+  subgoal 
+    by (smt INF_greatest Inf_lower image_eqI top_greatest) 
+  subgoal
+    apply(rule Inf_greatest)
+    apply auto apply(rule Inf_lower2)
+    by auto
+  done
+
+lemma If_Inf_commute: "(if b then Inf (f`G) else bot) \<le> Inf ((\<lambda>x. (if b then (f x)::ennreal else bot))`G) "
+  apply(cases b) by auto
+
+lemma If_Sup_commute_bot: "(if b then Sup (f`G) else bot) \<le> Sup ((\<lambda>x. (if b then (f x)::ennreal else bot))`G) "
+  apply(cases b) by auto
+lemma If_Sup_commute_top: "(if b then Sup (f`G) else top) \<ge> Sup ((\<lambda>x. (if b then (f x)::ennreal else top))`G) "
+  apply(cases b) by auto
+
+lemma tta: "(if b then x - y else bot) \<le> (if b then x else bot) - (y::ennreal)"
+  by(auto)
+
+
+thm ENNREAL_PLUS.Sup_mult_right_distrib
+
+
+lemma INF_ennreal_add_const_local2:
+  fixes f g :: "_ \<Rightarrow> ennreal"
+  shows "(INF i\<in>A. f i + c) = (INF i\<in>A. f i) + c"
+  apply(cases  "A={}")
+  subgoal by simp
+  subgoal 
+    using continuous_at_Inf_mono[of "\<lambda>x. x + c" "f`A"]
+    using continuous_add[of "at_right (Inf (f ` A))", of "\<lambda>x. x" "\<lambda>x. c"]
+    by (auto simp: image_comp mono_def) 
+  done
+
+thm continuous_diff
+thm continuous_add
+
+lemma "Inf (f`X) - c = Inf ((\<lambda>x. (f x::ennreal) - c)`X)"
+  apply(cases  "X={}")
+  subgoal by simp
+  subgoal 
+    oops
+
+
+text \<open>
+  The following lemma can also be stated using monotone functions @{term f} and  @{term g}. But then
+  the continuity assumption needs to be for all cardinals, not only countable.
+\<close>
+
+lemma lfp_parallel_induct[consumes 2, case_names bot step cont]:
+  assumes f: "sup_continuous f" and g: "sup_continuous g"
+  assumes bot: "R bot bot"
+  assumes step: "\<And>x y. R x y \<Longrightarrow> R (f x) (g y)"
+  assumes cont: "\<And>X Y. (\<And>i::nat. R (X i) (Y i)) \<Longrightarrow> mono X \<Longrightarrow> mono Y \<Longrightarrow> R (SUP i. X i) (SUP i. Y i)"
+  shows "R (lfp f) (lfp g)"
+  unfolding f[THEN sup_continuous_lfp] g[THEN sup_continuous_lfp]
+proof (rule cont)
+  show "incseq (\<lambda>i. (f ^^ i) bot)" "incseq (\<lambda>i. (g ^^ i) bot)"
+    by (intro mono_funpow f[THEN sup_continuous_mono] g[THEN sup_continuous_mono])+
+  show "R ((f ^^ i) bot) ((g ^^ i) bot)" for i
+    by (induction i) (auto intro: bot step)
+qed
+
+
+
+lemma ennreal_SUP_add_left_le:
+  fixes c :: ennreal
+  shows "(SUP i\<in>I. f i + c) \<le> (SUP i\<in>I. f i) + c"
+  apply(cases "I={}")
+   apply simp
+  apply(subst ennreal_SUP_add_left) apply auto
+  done
+
+lemma INF_ennreal_add_const:
+  fixes f g :: "_ \<Rightarrow> ennreal"
+  shows "(INF i. f i + c) = (INF i. f i) + c"
+  using continuous_at_Inf_mono[of "\<lambda>x. x + c" "f`UNIV"]
+  using continuous_add[of "at_right (Inf (range f))", of "\<lambda>x. x" "\<lambda>x. c"]
+  by (auto simp: mono_def image_comp)
+
+
+lemma INF_ennreal_const_add'':
+  fixes f  :: "_ \<Rightarrow> ennreal" 
+  shows " c + Inf (f`X) = Inf ((\<lambda>x. c + f x)`X)" 
+    using  INF_ennreal_const_add' by metis
+
+abbreviation "Supl \<equiv> ENNREAL_PLUS.INFI"
+abbreviation "Infl \<equiv> ENNREAL_PLUS.SUPR"
+
+
+definition "pt_m ae e = ((pt ae e)\<star>\<^sub>p(emb\<^sub>p (\<lambda>_. True)))"
+
+lemma lemmaB1: "((pt ae e) \<star>\<^sub>p ( (pt ae e) -\<star>\<^sub>p X)) = (pt_m ae e + X)"
+    
+
+  sorry
+
+lemma pt_m_reduce: "a ## b \<Longrightarrow> pt_m x2 e (s, a + b) \<le> pt_m x2 e (s, a)"
+  unfolding pt_m_def
+  unfolding star_pot_method_alt'' apply auto
+  apply(rule INF_mono) apply auto
+  subgoal for x y
+    apply(rule exI[where x=x])
+    apply(rule exI[where x="y+b"])
+    apply safe
+    subgoal using sep_add_assoc sep_add_disjD by blast 
+    subgoal using sep_disj_addI3 by auto 
+    subgoal by (simp add: emb\<^sub>p_alt)
+    done
+  done
+
+
+lemma ert_Lookup_alt': "ert (Lookup x ae) X =
+     ((\<lambda>(s,h). (INF val\<in>UNIV.  (pt_m ae (\<lambda>_. val) + (\<lambda>(s,h). X (s(x:=val),h))) (s,h))) \<star>\<^sub>p dollar 1)"
+  unfolding ert_Lookup_alt
+  apply(subst lemmaB1)   by auto
+
+
+lemma Inf_swap: "\<And>X f. Infl UNIV (\<lambda>u. Infl X (\<lambda>x. f u x)) = Infl X (\<lambda>x. Infl UNIV (\<lambda>u. f u x))"
+    using ENNREAL_PLUS.SUP_commute by blast 
+
+
+
+text \<open>Appendix B.12 in @{cite batzPOPL19}\<close>
+lemma quantitative_frame_rule: 
+  shows "Mod c \<inter> Vars \<Pi> = {} \<Longrightarrow> ert c (\<Psi> \<star>\<^sub>p \<Pi>) \<le> (ert c \<Psi> \<star>\<^sub>p \<Pi>)"
+proof (induct c arbitrary: \<Psi>)
+  case Skip
+  then show ?case
+    apply (simp add: plus_as_dollar_conv  ) 
+    apply(subst (2) star_pot_method_commute)
+    apply(subst (3) star_pot_method_commute)
+    apply(subst star_pot_method_assoc[symmetric]) 
+    by simp
+next
+  case (Assign x1 x2)
+  then show ?case 
+    apply (simp add: plus_as_dollar_conv  )
+    apply(rule le_funI)
+    apply auto
+    apply(subst Assign_propagates_star) apply simp
+    apply(subst (2) star_pot_method_commute)
+    apply(subst (3) star_pot_method_commute)
+    apply(subst star_pot_method_assoc[symmetric]) 
+    by simp
+next
+  case (Seq c1 c2)
+  then show ?case
+    apply (auto intro!: ert_mono)
+    apply (drule quantitative_frame_rule_aux)
+    apply(rule order.trans)
+     apply(rule ert_mono[where g="ert c2 \<Psi> \<star>\<^sub>p \<Pi>"])
+    by simp_all
+(*next
+  case (Coin c1 x2 c2)
+
+
+  {
+    fix a b
+    have "x2 * ert c1 (\<Psi> \<star>\<^sub>p \<Pi>) (a, b) + (1 - x2) * ert c2 (\<Psi> \<star>\<^sub>p \<Pi>) (a, b)
+         \<le> G" sorry
+    also have "\<dots> \<le> ((\<lambda>a. x2 * ert c1 \<Psi> a + (1 - x2) * ert c2 \<Psi> a) \<star>\<^sub>p \<Pi>) (a, b)"
+      sorry
+    also have "\<dots> \<le> ((\<lambda>a. x2 * ert c1 \<Psi> a + (1 - x2) * ert c2 \<Psi> a) \<star>\<^sub>p (x2 * \<Pi> + (1-x2) * \<Pi>)) (a, b)"
+      sorry
+    finally have "x2 * ert c1 (\<Psi> \<star>\<^sub>p \<Pi>) (a, b) + (1 - x2) * ert c2 (\<Psi> \<star>\<^sub>p \<Pi>) (a, b)
+       \<le> ((\<lambda>a. x2 * ert c1 \<Psi> a + (1 - x2) * ert c2 \<Psi> a) \<star>\<^sub>p \<Pi>) (a, b)"
+      .
+  }
+
+  from Coin show ?case
+    apply (auto simp: le_fun_def) 
+    using theorem_3_11_3
+    apply(rule add_mono)
+    sorry *)
+next
+  case (If x1 c1 c2)
+  then show ?case
+    unfolding ert_If_alt Mod.simps
+    apply -
+    apply (drule quantitative_frame_rule_aux)
+    apply(rule order.trans[OF _ sub_distributivity_of_star_over_inf'])
+    apply(subst theorem_3_11_3')
+    subgoal 
+      unfolding emb\<^sub>p_alt pure\<^sub>p_alt by auto
+    apply(subst theorem_3_11_3')
+    subgoal 
+      unfolding emb\<^sub>p_alt pure\<^sub>p_alt by auto
+    apply(rule inf_mono)
+    subgoal 
+     (* supply [[unify_trace_failure]] *)
+      apply(rule le_funI)
+      apply(simp only: plus_fun_def)
+      apply(rule add_left_mono) by (auto simp add: le_fun_def)  
+    subgoal 
+     (* supply [[unify_trace_failure]] *)
+      apply(rule le_funI)
+      apply(simp only: plus_fun_def)
+      apply(rule add_left_mono) by (auto simp add: le_fun_def)  
+    done
+next
+  case (While x1 c)
+
+  let ?f = "(\<lambda>Y (s, h). 1 + (if x1 s then ert c Y (s, h) else (\<Psi> \<star>\<^sub>p \<Pi>) (s, h)))"
+  let ?g = "(\<lambda>Y (s, h). 1 + (if x1 s then ert c Y (s, h) else \<Psi> (s, h)))"
+  have fg: "mono ?f" "mono ?g" 
+    by (auto intro!: monoI ert_mono le_funI ert_mono[THEN le_funD])
+
+  thm lfp_lockstep_induct[where f="?f"]
+
+  show ?case
+    apply clarsimp
+  proof(induct rule: lfp_lockstep_induct[where f="?f" and g="?g"])
+    case monof
+    then show ?case using fg by simp
+  next
+    case monog
+    then show ?case using fg by simp
+  next
+    case (step A B)
+     
+    have *: "\<And>a b. Inf {ert c B (a, x) + \<Pi> (a, y) |x y. b = x + y \<and> x ## y}
+        = Inf ((\<lambda>(x,y). ert c B (a, x) + \<Pi> (a, y))`{(x,y)|x y. b = x + y \<and> x ## y})"
+      apply(rule arg_cong[where f=Inf]) by auto
+    have **: "\<And>a b. Inf {1+ ert c B (a, x) + \<Pi> (a, y) |x y. b = x + y \<and> x ## y}
+        = Inf ((\<lambda>(x,y). 1+ ert c B (a, x) + \<Pi> (a, y))`{(x,y)|x y. b = x + y \<and> x ## y})"
+      apply(rule arg_cong[where f=Inf]) by auto
+    have ***: "\<And>a b. Inf {\<Psi> (a, x) + \<Pi> (a, y) |x y. b = x + y \<and> x ## y}
+            = Inf ((\<lambda>(x,y). \<Psi> (a, x) + \<Pi> (a, y))`{(x,y)|x y. b = x + y \<and> x ## y})"
+      apply(rule arg_cong[where f=Inf]) by auto
+    have ****: "\<And>a b. Inf {1 + \<Psi> (a, x) + \<Pi> (a, y) |x y. b = x + y \<and> x ## y}
+            = Inf ((\<lambda>(x,y). 1 + \<Psi> (a, x) + \<Pi> (a, y))`{(x,y)|x y. b = x + y \<and> x ## y})"
+      apply(rule arg_cong[where f=Inf]) by auto
+    show ?case
+      apply -
+      apply (rule le_funI)
+      apply auto
+       apply(rule order.trans)
+        apply(rule add_left_mono) 
+      apply(rule ert_mono')  
+         apply(rule step(3))
+       apply(rule order.trans)
+        apply(rule add_left_mono)   
+        apply(rule While(1)[THEN le_funD])
+      subgoal using While(2) by auto
+      subgoal unfolding star_pot_method_alt
+        apply auto
+        unfolding *
+        apply(subst INF_ennreal_const_add'') 
+        unfolding **    
+        apply(rule INF_mono) by force 
+      subgoal unfolding star_pot_method_alt
+        apply auto
+        unfolding ***
+        apply(subst INF_ennreal_const_add'') 
+        unfolding ****   
+        apply(rule INF_mono) by force 
+      done
+  next
+    case (union M)
+    show ?case 
+      unfolding fst_proj_def snd_proj_def 
+      apply(rule Sup_least) apply auto
+      subgoal for A B
+        using union[rule_format, of "(A,B)"] apply simp
+        apply(rule order.trans)
+         apply(assumption)
+        apply(rule le_funI)
+        apply(rule star_pot_method_mono) apply(rule Sup_upper) by auto
+      done
+  qed
+next
+  case (New x1 x2)
+  then have tt: "\<And>y a ma . \<Pi> (a(x1 := ma), y)  = \<Pi> (a, y)"
+    by (simp add: not_in_Vars_upd_okay) 
+
+  show ?case
+    unfolding ert_New_alt
+    apply(rule le_funI)  
+    apply(subst (1) star_pot_method_assoc[symmetric])
+    apply(subst (4) star_pot_method_commute)
+    apply(subst (1) star_pot_method_assoc)
+    apply(rule star_pot_method_mono[rotated]) apply simp
+    apply simp
+    apply(case_tac sh) apply simp
+  proof -
+    fix s h
+    have " Supl UNIV (\<lambda>a. ([(\<lambda>_. a) \<mapsto> x2] -\<star>\<^sub>p (\<lambda>(s, h). (\<Psi> \<star>\<^sub>p \<Pi>) (s(x1 := a), h))) (s,h))
+        \<le> Supl UNIV (\<lambda>x. ([(\<lambda>_. x) \<mapsto> x2] -\<star>\<^sub>p
+             (\<lambda>(s, h). Infl {(x, y). h = x + y \<and> x ## y}
+                               (\<lambda>(xa, y). \<Psi> (s(x1 := x), xa) + \<Pi> (s(x1 := x), y))))  (s,h))"
+      unfolding star_pot_method_alt'' by simp
+    also have "\<dots> \<le> Supl UNIV (\<lambda>x. ([(\<lambda>_. x) \<mapsto> x2] -\<star>\<^sub>p (\<lambda>(s, h). Infl {(x, y). h = x + y \<and> x ## y} (\<lambda>(xa, y). \<Psi> (s(x1 := x), xa) + \<Pi> (s, y))))  (s,h))"
+      apply(subst tt) by simp
+    also have "\<dots> \<le>  Supl UNIV (\<lambda>x. Supl {h'. h ## h' \<and> ptb (\<lambda>_. x) x2 (s, h')}
+                   (\<lambda>h'. Infl {(h1, h2). h + h' = h1 + h2 \<and> h1 ## h2} (\<lambda>(h1, h2). \<Psi> (s(x1 := x), h1) + \<Pi> (s, h2))))"
+      unfolding pt_emb  wand_pot_method_emb_alt by simp
+    also have "\<dots> \<le>  Supl UNIV (\<lambda>x. Supl {h'. h ## h' \<and> ptb (\<lambda>_. x) x2 (s, h')}
+                       (\<lambda>h'. Infl {(h1, h2). h = h1 + h2 \<and> h1 ## h2} (\<lambda>(h1, h2). \<Psi> (s(x1 := x), h1 + h') + \<Pi> (s, h2))))"
+      \<comment> \<open>choose h' \<subseteq> h1\<close>
+      apply(rule SUP_mono)
+      apply auto
+      subgoal for x
+        apply(rule exI[where x=x])
+        apply(rule SUP_mono) apply auto
+        subgoal for h' 
+          apply(rule exI[where x="h'"]) apply auto
+          apply(rule INF_mono) apply auto
+          subgoal for a b apply(rule exI[where x="a + h'"])
+            apply(rule exI[where x="b"]) apply auto
+            subgoal
+              by (metis sep_add_assoc sep_add_commute sep_add_disjD sep_add_disjI1)  
+            subgoal 
+              using sep_add_disjI1 by blast  
+            done
+          done
+        done
+      done
+    also have "\<dots>  \<le> Infl {(x, y). h = x + y \<and> x ## y} (\<lambda>x. case x of (x, y) \<Rightarrow> Supl UNIV (\<lambda>xa. Supl {h'. x ## h' \<and> ptb (\<lambda>_. xa) x2 (s, h')} (\<lambda>xaa. \<Psi> (s(x1 := xa), x + xaa)+ \<Pi> (s, y))) )"
+      apply(rule order.trans)
+       apply(rule SUP_mono') 
+       apply(rule qfr_aux1)
+      apply(rule order.trans) 
+       apply(rule qfr_aux1)
+      apply(rule INF_mono)
+      subgoal for m
+        apply(rule bexI[where x=m])  apply auto
+        apply(rule SUP_mono) apply auto
+        subgoal for x y a apply(rule exI[where x=a])
+          apply(rule Sup_mono)
+          apply auto
+          using sep_add_disjD by blast   
+        done
+      done
+    also have "\<dots>  \<le> Infl {(x, y). h = x + y \<and> x ## y} (\<lambda>x. case x of (x, y) \<Rightarrow> Supl UNIV (\<lambda>xa. Supl {h'. x ## h' \<and> ptb (\<lambda>_. xa) x2 (s, h')} (\<lambda>xaa. \<Psi> (s(x1 := xa), x + xaa))) + \<Pi> (s, y))"
+      apply(rule INF_mono)
+      subgoal for m
+        apply(rule bexI[where x=m])  
+         apply auto
+        apply(rule order.trans[rotated])
+         apply(rule ennreal_SUP_add_left_le)    
+        apply(rule SUP_mono)
+        subgoal for x y u
+          apply(rule bexI[where x=u])  apply auto
+          apply(rule ennreal_SUP_add_left_le) done
+        done
+      done
+   
+    also have "\<dots>  \<le> Infl {(x, y). h = x + y \<and> x ## y} (\<lambda>x. case x of (x, y) \<Rightarrow> Supl UNIV (\<lambda>a. ([(\<lambda>_. a) \<mapsto> x2] -\<star>\<^sub>p (\<lambda>(s, h). \<Psi> (s(x1 := a), h))) (s, x)) + \<Pi> (s, y))"
+      unfolding pt_emb  wand_pot_method_emb_alt apply simp done
+    also have "\<dots>  \<le> ((\<lambda>(s, h). Supl UNIV (\<lambda>a. ([(\<lambda>_. a) \<mapsto> x2] -\<star>\<^sub>p (\<lambda>(s, h). \<Psi> (s(x1 := a), h))) (s, h))) \<star>\<^sub>p \<Pi>)  (s,h)"
+      unfolding star_pot_method_alt'' apply simp done
+    finally show " Supl UNIV (\<lambda>a. ([(\<lambda>_. a) \<mapsto> x2] -\<star>\<^sub>p (\<lambda>(s, h). (\<Psi> \<star>\<^sub>p \<Pi>) (s(x1 := a), h)))  (s,h))
+         \<le> ((\<lambda>(s, h). Supl UNIV (\<lambda>a. ([(\<lambda>_. a) \<mapsto> x2] -\<star>\<^sub>p (\<lambda>(s, h). \<Psi> (s(x1 := a), h))) (s, h))) \<star>\<^sub>p \<Pi>)  (s,h)"
+      .
+  qed
+   
+
+ 
+next
+  case (Free x)
+  then show ?case
+    apply simp
+    apply(rule le_funI)
+    unfolding plus_as_dollar_conv' plus_as_dollar_conv
+    by(auto simp: star_pot_method_commute star_pot_method_commute_c)
+next
+  case (Lookup x1 x2)
+  then have tt: "\<And>y a ma . \<Pi> (a(x1 := ma), y)  = \<Pi> (a, y)"
+    by (simp add: not_in_Vars_upd_okay) 
+
+
+  show ?case
+    unfolding ert_Lookup_alt'
+    apply(rule le_funI) 
+    apply(subst (1) star_pot_method_assoc[symmetric])
+    apply(subst (4) star_pot_method_commute)
+    apply(subst (1) star_pot_method_assoc)
+    apply(rule star_pot_method_mono[rotated]) apply simp
+    apply auto
+  proof -
+    fix s h
+    have "Infl UNIV (\<lambda>x. pt_m x2 (\<lambda>_. x) (s, h) + (\<Psi> \<star>\<^sub>p \<Pi>) (s(x1 := x), h))
+        \<le> Infl UNIV (\<lambda>x. pt_m x2 (\<lambda>_. x) (s, h) + Infl {(x, y). h = x + y \<and> x ## y} (\<lambda>(xa, y). \<Psi> (s(x1 := x), xa) + \<Pi> (s(x1 := x), y)))"
+      unfolding star_pot_method_alt'' apply simp done
+    also have "\<dots> \<le>
+         Infl UNIV (\<lambda>x. pt_m x2 (\<lambda>_. x) (s, h) + Infl {(x, y). h = x + y \<and> x ## y} (\<lambda>(xa, y). \<Psi> (s(x1 := x), xa) + \<Pi> (s, y)))"
+      apply(subst tt) apply simp done
+    also have "\<dots> \<le> Infl UNIV (\<lambda>x. Infl {(x, y). h = x + y \<and> x ## y} (\<lambda>(h1,h2). (pt_m x2 (\<lambda>_. x) (s, h) + (\<Psi> (s(x1 := x), h1)) + \<Pi> (s, h2))))"
+      \<comment> \<open>Algebra\<close>
+      apply(subst INF_ennreal_const_add'') 
+      apply(simp only: split_beta) apply(rule INF_mono') apply(rule INF_mono') by auto
+    also have "\<dots> \<le> Infl UNIV (\<lambda>x. Infl {(x, y). h = x + y \<and> x ## y} (\<lambda>(h1,h2). (pt_m x2 (\<lambda>_. x) (s, h1) + (\<Psi> (s(x1 := x), h1)) + \<Pi> (s, h2))))"
+      \<comment> \<open>take subset in which [pt_m] is evaluated in h1 instead of h\<close>
+      apply(rule INF_mono) apply auto
+      subgoal for u apply(rule exI[where x=u]) 
+      apply(rule INF_mono) apply auto
+        subgoal for a b 
+          apply(rule exI[where x=a])
+          apply(rule exI[where x=b])
+          apply safe apply(rule add_right_mono)
+          apply(rule add_right_mono)
+          apply(rule pt_m_reduce) by simp
+        done
+      done
+    also have "\<dots> \<le> Infl {(x, y). h = x + y \<and> x ## y} (\<lambda>x. case x of (x, y) \<Rightarrow> Infl UNIV (\<lambda>xa. pt_m x2 (\<lambda>_. xa) (s, x) + \<Psi> (s(x1 := xa), x)) + \<Pi> (s, y))"
+      apply(subst Inf_swap)
+      apply(rule INF_mono') apply auto
+      apply(subst INF_ennreal_add_const)
+      by auto 
+    also have "\<dots> \<le> ((\<lambda>(s, h). Infl UNIV (\<lambda>x. pt_m x2 (\<lambda>_. x) (s, h) + \<Psi> (s(x1 := x), h))) \<star>\<^sub>p \<Pi>)  (s, h)"
+      unfolding star_pot_method_alt'' apply simp done
+    finally show "Infl UNIV (\<lambda>x. pt_m x2 (\<lambda>_. x) (s, h) + (\<Psi> \<star>\<^sub>p \<Pi>) (s(x1 := x), h))
+         \<le> ((\<lambda>(s, h). Infl UNIV (\<lambda>x. pt_m x2 (\<lambda>_. x) (s, h) + \<Psi> (s(x1 := x), h))) \<star>\<^sub>p \<Pi>) (s, h)"
+      .
+  qed
+next
+  case (Update x1 x2) 
+  
+  have *: "\<And>x. (([x1 \<mapsto> x2] -\<star>\<^sub>p \<Psi> \<star>\<^sub>p \<Pi>)) x \<le> (\<Pi> \<star>\<^sub>p ([x1 \<mapsto> x2] -\<star>\<^sub>p \<Psi>)) x"
+    apply(case_tac x) apply simp
+  proof -
+    fix s h
+    have "(([x1 \<mapsto> x2] -\<star>\<^sub>p \<Psi> \<star>\<^sub>p \<Pi>)) (s,h)
+       = Supl {h'. h ## h' \<and> ptb x1 x2 (s, h')} (\<lambda>h'. (\<Psi> \<star>\<^sub>p \<Pi>) (s, h + h'))"
+      unfolding pt_emb  wand_pot_method_emb_alt by simp
+    also have "\<dots> = Supl {h'. h ## h' \<and> ptb x1 x2 (s, h')}
+                          (\<lambda>h'. Infl {(x, y). h + h' = x + y \<and> x ## y}
+                            (\<lambda>(x, y). \<Psi> (s, x) + \<Pi> (s, y)))" 
+      unfolding star_pot_method_alt''  by simp
+
+    also have "\<dots> \<le> Supl {h'. h ## h' \<and> ptb x1 x2 (s, h')}
+                          (\<lambda>h'. Infl {(h1, h2). h = h1 + h2 \<and> h1 ## h2}
+                            (\<lambda>(h1, h2). \<Psi> (s, h1 + h') + \<Pi> (s, h2)))" 
+      \<comment> \<open>choose h' \<subseteq> h1\<close> (* the same step as in the New case, maybe factor it out? *)
+      apply(rule SUP_mono)
+      apply auto
+      subgoal for h'
+        apply(rule exI[where x=h']) apply simp
+        apply(rule INF_mono) apply auto
+        subgoal for a b apply(rule exI[where x="a + h'"])
+          apply(rule exI[where x="b"]) apply auto
+          subgoal
+            by (metis sep_add_assoc sep_add_commute sep_add_disjD sep_add_disjI1)  
+          subgoal 
+            using sep_add_disjI1 by blast  
+          done
+        done
+      done
+
+    also have "\<dots> \<le> Infl {(h1, h2). h = h1 + h2 \<and> h1 ## h2} 
+                          (\<lambda>x. case x of (h1, h2) \<Rightarrow> 
+                                   Supl {h'. h1 ## h' \<and> ptb x1 x2 (s, h')} (\<lambda>h'. \<Psi> (s, h1 + h') + \<Pi> (s, h2)) ) " 
+
+      apply(rule order.trans) 
+       apply(rule qfr_aux1)
+      apply(rule INF_mono)
+      subgoal for m apply(rule bexI[where x=m])  apply auto
+        apply(rule SUP_mono) apply auto
+        subgoal for x y a apply(rule exI[where x=a]) apply auto  
+          using sep_add_disjD by blast   
+        done
+      done
+       
+    also have "\<dots> \<le> Infl {(h1, h2). h = h1 + h2 \<and> h1 ## h2} 
+                          (\<lambda>x. case x of (h1, h2) \<Rightarrow> 
+                                   Supl {h'. h1 ## h' \<and> ptb x1 x2 (s, h')} (\<lambda>h'. \<Psi> (s, h1 + h')) + \<Pi> (s, h2)) "
+      apply(rule INF_mono')
+      apply auto
+      by(rule ennreal_SUP_add_left_le)
+    also have "\<dots> = Infl {(x, y). h = x + y \<and> x ## y} (\<lambda>x. case x of (x, y) \<Rightarrow> ([x1 \<mapsto> x2] -\<star>\<^sub>p \<Psi>) (s, x) + \<Pi> (s, y) )"
+      unfolding pt_emb  wand_pot_method_emb_alt by simp
+    also have "\<dots> = (([x1 \<mapsto> x2] -\<star>\<^sub>p \<Psi>) \<star>\<^sub>p \<Pi>) (s,h)"
+      unfolding star_pot_method_alt'' by simp
+    also have "\<dots> = (\<Pi> \<star>\<^sub>p ([x1 \<mapsto> x2] -\<star>\<^sub>p \<Psi>)) (s,h)"
+      apply(subst star_pot_method_commute) by simp
+    finally show "(([x1 \<mapsto> x2] -\<star>\<^sub>p \<Psi> \<star>\<^sub>p \<Pi>)) (s,h) \<le> (\<Pi> \<star>\<^sub>p ([x1 \<mapsto> x2] -\<star>\<^sub>p \<Psi>)) (s,h)"
+      by simp
+  qed
+    
+
+  show ?case
+    apply simp
+    apply(rule le_funI)
+    unfolding plus_as_dollar_conv' plus_as_dollar_conv 
+    using star_pot_method_commute_c
+    apply(subst (1) star_pot_method_assoc[symmetric])
+    apply(subst (2) star_pot_method_assoc[symmetric])
+    apply(subst star_pot_method_assoc[symmetric])
+    apply(rule star_pot_method_mono) apply simp
+    apply(subst (2) star_pot_method_commute)
+    apply(subst (3) star_pot_method_commute)
+    apply(subst  star_pot_method_assoc[symmetric])
+    apply(rule star_pot_method_mono) apply simp
+    apply(rule *) done
+qed
+
+
+
+lemma Frame_rule:
+  assumes "Hoare_triple \<Phi> c \<Psi>"
+  and "Mod c \<inter> Vars \<Pi> = {}"
+  shows "Hoare_triple (\<Phi> \<star>\<^sub>p \<Pi>) c (\<Psi> \<star>\<^sub>p \<Pi>)"
+proof 
+  have "ert c (\<Psi> \<star>\<^sub>p \<Pi>) \<le> ((ert c \<Psi>) \<star>\<^sub>p \<Pi>)"
+    apply(rule quantitative_frame_rule)
+    by fact
+  also have "\<dots> \<le> (\<Phi> \<star>\<^sub>p \<Pi>)"
+    apply(rule le_funI)
+    apply(rule star_pot_method_mono)
+    subgoal using assms(1)[THEN Hoare_tripleD] using le_fun_def by metis
+    by simp
+  finally show "ert c (\<Psi> \<star>\<^sub>p \<Pi>) \<le> (\<Phi> \<star>\<^sub>p \<Pi>)" .
+qed
+    
+
 
 
 
@@ -449,21 +1233,6 @@ definition pureassn\<^sub>p :: "(stack \<Rightarrow> bool) \<Rightarrow> stack \
 lemma pureassn\<^sub>p_True_emp_conv: "pureassn\<^sub>p (\<lambda>_. True) = sep_empty\<^sub>p"
   unfolding   sep_empty\<^sub>p_alt pureassn\<^sub>p_def emb\<^sub>p_alt by auto
 
-definition dollar where
-  "dollar c = (\<lambda>(s,h). if h=0 then c else \<infinity>)"
-
-lemma plus_as_dollar_conv: "\<And>Q a c. Q a + c = (Q \<star>\<^sub>p dollar c) a"  
-  unfolding dollar_def star_pot_method_alt''
-  apply auto
-  apply(rule antisym)
-  subgoal apply(rule Inf_greatest) apply auto  
-    by (simp add: add_top)  
-  subgoal for Q a b apply(rule Inf_lower)
-    apply ( rule image_eqI[where x="(b,0)"]) apply simp apply simp done
-  done
-
-lemma plus_as_dollar_conv': "\<And>Q. (\<lambda>a. Q a + c) = (Q \<star>\<^sub>p dollar c)"  
-  apply (rule ext) by(rule plus_as_dollar_conv)
 
 
 lemma "pure\<^sub>p (pureassn\<^sub>p A)"
